attic/BasicBlocks.thy
@@ -35,6 +35,7 @@ type_synonym stack_value = "w256 option"
 record basic_blocks =
 blocks_indexes :: "int list"
 blocks_list :: "int \<Rightarrow> vert option"
+all_blocks :: "vertices"
 
 (* Auxiliary functions *)
 
@@ -131,32 +132,12 @@ definition build_blocks :: "inst list \<Rightarrow> basic_blocks" where
 "build_blocks prog = (let blocks = build_vertices prog in
 (let ind = (extract_indexes blocks) in
 (|blocks_indexes = ind,
-  blocks_list = map_of blocks|)
+  blocks_list = map_of blocks,
+  all_blocks = blocks|)
 ))"
 
 (* Verification *)
 lemmas reg_inst_splits = inst.splits misc_inst.splits pc_inst.splits
-
-(* Check that we can rebuild the initial list of instructions from basic blocks *)
-fun reconstruct_bytecode :: "vertices \<Rightarrow> inst list" where
- "reconstruct_bytecode [] = []"
-| "reconstruct_bytecode ((n,b,Jump)#q) = (map snd b)@[Pc JUMP] @ (reconstruct_bytecode q)"
-| "reconstruct_bytecode ((n,b,Jumpi)#q) = (map snd b)@[Pc JUMPI] @ (reconstruct_bytecode q)"
-| "reconstruct_bytecode ((n,b,_)#q) = (map snd b) @ (reconstruct_bytecode q)"
-
-lemma rev_basic_blocks: "reconstruct_bytecode (aux_basic_block i b) = (map snd b)@(map snd i)"
-apply(induction i arbitrary: b)
-apply(case_tac b)
-apply(auto simp: Let_def aux_basic_block.simps split: reg_inst_splits)
-done
-
-lemma remove_address:
-"map snd (add_address' i k) = i"
-by(induction i arbitrary: k; simp)
-
-theorem reverse_basic_blocks: "reconstruct_bytecode (build_vertices i) = i"
-apply(simp add: rev_basic_blocks build_vertices_def add_address_def remove_address)
-done
 
 (* Define how BLOCKSs should be for the program logic to be sound *)
 
@@ -190,51 +171,6 @@ declare seq_block.simps[simp del]
 definition last_no::"pos_inst list \<Rightarrow> bool" where
 "last_no insts == snd (last insts) \<in> {Misc STOP, Misc RETURN, Misc SUICIDE}"
 
-(* Define a 'program' from a BLOCKS *)
-
-fun blocks_insts_aux :: "basic_blocks \<Rightarrow> int list \<Rightarrow> pos_inst list" where
-  "blocks_insts_aux c [] = []"
-| "blocks_insts_aux c (x#xs) = (case blocks_list c x of
-    None \<Rightarrow> blocks_insts_aux c xs
-  | Some (b,_) \<Rightarrow> b @ (blocks_insts_aux c xs))"
-
-definition blocks_insts :: "basic_blocks \<Rightarrow> pos_inst set" where
-"blocks_insts c = set (blocks_insts_aux c (blocks_indexes c))"
-
-fun inst_size_list::"pos_inst list \<Rightarrow> int" where
-"inst_size_list [] = 0"
-| "inst_size_list (x#xs) = inst_size (snd x) + inst_size_list xs"
-
-fun blocks_pos_insts :: "vertices \<Rightarrow> pos_inst list" where
- "blocks_pos_insts [] = []"
-| "blocks_pos_insts ((n,b,Jump)#q) = b@[(n+inst_size_list b,Pc JUMP)] @ (blocks_pos_insts q)"
-| "blocks_pos_insts ((n,b,Jumpi)#q) = b@[(n+inst_size_list b,Pc JUMPI)] @ (blocks_pos_insts q)"
-| "blocks_pos_insts ((n,b,_)#q) = b @ (blocks_pos_insts q)"
-
-fun blocks_vertices:: "basic_blocks \<Rightarrow> int list \<Rightarrow> vertex list" where
-"blocks_vertices c [] = []"
-| "blocks_vertices c (x#xs) = (case blocks_list c x of
-  None \<Rightarrow> blocks_vertices c xs
-  | Some b \<Rightarrow> (x,b) # (blocks_vertices c xs))"
-
-definition blocks_content ::"basic_blocks \<Rightarrow> int \<Rightarrow> inst option " where
-"blocks_content c  = map_of (blocks_pos_insts (blocks_vertices c (blocks_indexes c)))"
-
-definition blocks_length :: "basic_blocks \<Rightarrow> int " where
-"blocks_length c =
-  (case blocks_list c (last (blocks_indexes c)) of
-    None \<Rightarrow> 0 (*Should not happen*)
-  | Some (i,Jump) \<Rightarrow> fst (last i) +  inst_size (snd (last i))
-  | Some (i,Jumpi) \<Rightarrow> fst (last i) + inst_size (snd (last i))
-  | Some (i,_) \<Rightarrow> fst (last i))"
-
-definition program_from_blocks:: "basic_blocks \<Rightarrow> program" where
-"program_from_blocks c = ( (|
-  program_content = blocks_content c,
-  program_length = blocks_length c,
-  program_annotation = (\<lambda> _ .  [])
-|) )"
-
 definition wf_blocks:: "basic_blocks \<Rightarrow> bool" where
 "wf_blocks c == 
 (\<forall>n insts ty.
@@ -244,13 +180,11 @@ definition wf_blocks:: "basic_blocks \<Rightarrow> bool" where
   0 \<le> n \<and> n < 2 ^ 256) \<and>
 (blocks_list c n = Some (insts, Next) \<longrightarrow>
 	 insts \<noteq> []) \<and>
-(blocks_list c n = Some (insts, Jump) \<longrightarrow>
-	program_content (program_from_blocks c) (n + inst_size_list insts) = Some (Pc JUMP)) \<and>
-(blocks_list c n = Some (insts, Jumpi) \<longrightarrow>
-	program_content (program_from_blocks c) (n + inst_size_list insts) = Some (Pc JUMPI)) \<and>
 (blocks_list c n = Some (insts, No) \<longrightarrow>
 	 insts \<noteq> [] \<and> last_no insts)
-)"
+) \<and>
+blocks_list c = map_of (all_blocks c) \<and>
+blocks_indexes c = extract_indexes (all_blocks c)"
 
 (* Proof that we build well formed BLOCKSs *)
 
@@ -470,383 +404,15 @@ apply(simp split: reg_inst_splits if_splits)
   apply(erule disjE; simp add: last_no_def)+
 done
 
-(*Draft*)
-lemma seq_block_sumC:
-"seq_block ((i,j) # list @ (a, b) # xs) \<Longrightarrow>
- i + (inst_size j + inst_size_list list) = a"
-apply(induction list arbitrary: i j; clarsimp)
- apply(simp add: seq_block.simps)
-apply(simp add: seq_block.simps)
-apply(fastforce)
-done
-
-lemma rev_basic_blocks_add:
-"seq_block (b@i) \<Longrightarrow> 
-blocks_pos_insts (aux_basic_block i b) = b@i"
-apply(induction i arbitrary: b)
- apply(case_tac b)
-  apply(simp add: aux_basic_block.simps)
- apply(simp add: aux_basic_block.simps)
-apply(simp add: aux_basic_block.simps Let_def)
-apply(case_tac b; clarsimp)
- apply(case_tac "reg_inst b")
-  apply(drule_tac x="[(a, b)]" in meta_spec; simp)
-  apply(case_tac b; simp; rename_tac x; case_tac x; simp)
- apply(drule_tac x="[]" in meta_spec; simp)
- apply(case_tac b; simp; rename_tac x; case_tac x; simp add: block_pt_def seq_block_tl)
-apply(case_tac "reg_inst b \<and> b \<noteq> Pc JUMPDEST")
- apply(drule_tac x="(((aa, bb) # list) @ [(a, b)])" in meta_spec; simp)
- apply(case_tac b; simp; rename_tac x; case_tac x; simp)
-apply(case_tac "b=Pc JUMPDEST")
- apply(drule_tac x="[(a, b)]" in meta_spec; simp)
- apply(drule meta_mp)
-  apply(simp add: seq_block_tl'[where xs="_ # _"])
- apply(assumption)
-apply(drule_tac x="[]" in meta_spec; simp)
-apply(subgoal_tac "seq_block ((a, b) # i)")
-apply(case_tac b; simp; rename_tac x; case_tac x; simp add: block_pt_def seq_block_tl seq_block_sumC)
-apply(simp add: seq_block_tl'[where xs="_ # _"])
-done
-
-lemma reverse_basic_blocks_add: 
- "blocks_pos_insts (aux_basic_block (add_address i) []) = (add_address i)"
-apply(subst rev_basic_blocks_add)
- apply(simp add: seq_block_add_address add_address_def)
-apply(simp)
-done
-
-(* Draft Jump *)
-
-lemma blocks_vert_rebuild_one:
-"distinct (map fst zs) \<Longrightarrow>
-(n,i) \<in> set zs \<Longrightarrow>
- blocks_vertices
-  \<lparr>blocks_indexes = (map fst zs), blocks_list = map_of zs\<rparr>
-  [n] = [(n,i)]"
-by simp
-
-lemma blocks_vert_rebuild_subset:
-"distinct (map fst zs) \<Longrightarrow>
- set xs \<subseteq> set zs \<Longrightarrow>
- blocks_vertices
-  \<lparr>blocks_indexes = (map fst zs), blocks_list = map_of zs\<rparr>
-  (map fst xs) = xs"
-apply(induction xs; simp)
-apply(erule conjE)
-apply(split option.split; rule conjI; simp)
- apply(rule_tac x="v_insts a" in exI; rule_tac x="v_ty a" in exI)
- apply(clarsimp)
-apply(clarsimp)
-apply(simp add: distinct_map inj_on_def)
-apply(fastforce)
-done
-
-lemma blocks_vert_rebuild:
-"distinct (map fst zs) \<Longrightarrow>
- blocks_vertices
-  \<lparr>blocks_indexes = (map fst zs), blocks_list = map_of zs\<rparr>
-  (map fst zs) = zs"
-by(simp add: blocks_vert_rebuild_subset)
-
-lemma add_address_greater:
-"(n,m) \<in> set (add_address' xs k) \<Longrightarrow>
-n \<ge> k"
-apply(induction xs arbitrary: k)
- apply(simp)
-apply(simp; erule disjE)
- apply(simp)
-apply(drule_tac x="k + inst_size a" in meta_spec)
-apply(simp add: inst_size_pos)
-apply(subgoal_tac "k + inst_size a \<ge> k")
- apply(simp)
-apply(simp add: inst_size_pos Orderings.order_class.order.strict_implies_order)
-done
-
-lemma remdups_id_add_address:
-"remdups (add_address' xs n) = (add_address' xs n)"
-apply(induction xs arbitrary: n)
- apply(simp)
-apply(clarsimp)
-apply(drule add_address_greater; simp)
-apply(drule linorder_class.leD; simp add: inst_size_pos)
-done
-
-lemma distinct_add_address:
-"distinct (map fst (add_address' xs n))"
-apply(simp add: distinct_map)
-apply(rule conjI)
- apply(insert remdups_id_add_address[where xs=xs and n=n]; simp)
-apply(clarsimp simp add: inj_on_def)
-apply(induction xs arbitrary: n)
- apply(simp)
-apply(simp)
-apply(erule disjE; erule disjE)
-   apply(fastforce)
-  apply(drule add_address_greater; simp)
-  apply(drule linorder_class.leD; simp add: inst_size_pos)
- apply(drule add_address_greater; simp)
- apply(drule linorder_class.leD; simp add: inst_size_pos)
-apply(fastforce)
-done
-
-lemma hd_inst_in_aux_bb:
-"(n,(n,x)#zs,t) \<in> set (aux_basic_block xs ys) \<Longrightarrow>
-(n, x) \<in> set ys \<or> (n, x) \<in> set xs"
-apply(induction xs arbitrary: ys)
- apply(case_tac ys; clarsimp simp add: aux_basic_block.simps)
-apply(simp add: aux_basic_block.simps Let_def)
-apply(case_tac "reg_inst (snd a) \<and> (snd a) \<noteq> Pc JUMPDEST")
- apply(simp split: reg_inst_splits; fastforce)
-apply(case_tac "snd a = Pc JUMPDEST")
- apply(simp split: reg_inst_splits if_splits)
-  apply(fastforce)
- apply(erule disjE)
-  apply(drule conjunct2; rule disjI1; clarsimp)
- apply(fastforce)
-apply(drule meta_spec[where x="[]"])
-apply(simp split: reg_inst_splits if_splits)
-    apply(erule disjE; clarsimp; case_tac ys; clarsimp)+
-done
-
-lemma inst_size_list_pos:
-"inst_size_list xs \<ge> 0"
-apply(induction xs; simp)
-apply(insert inst_size_pos)
-apply(drule_tac x="snd a" in meta_spec)
-apply(fastforce)
-done
-
-lemma seq_block_smaller:
-"seq_block (a # list @ (m, j) # xs) \<Longrightarrow>
-fst a < m "
- apply(case_tac a; clarsimp)
- apply(drule seq_block_sumC)
- apply(drule sym[where s="_+_"]; simp)
- apply(subgoal_tac "inst_size b + inst_size_list list \<ge> inst_size b")
-  apply(drule Orderings.order_class.dual_order.strict_trans1[where c=0])
-   apply(simp add: inst_size_pos)
-  apply(assumption)
- apply(simp add: inst_size_list_pos)
-done
-
-lemma seq_block_smaller_all:
-"seq_block (a # list @ (m, j) # xs) \<Longrightarrow>
-fst a < m \<and> (\<forall>x \<in> set xs. fst a < fst x)"
-apply(rule conjI)
- apply(simp add: seq_block_smaller)
-apply(clarsimp)
-apply(subgoal_tac "\<exists>ys zs. xs = ys @ (aa, b) # zs")
- apply(clarify)
- apply(simp add: seq_block_smaller[where list="list @ (m,j)#_"])
-apply(thin_tac "seq_block _")
-apply(induction xs; simp)
-apply(erule disjE)
- apply(fastforce)
-apply(drule_tac x="aa" and y=b in meta_spec2; clarsimp)
-apply(rule_tac x="(a, b) # ys" in exI; simp)
-done
-
-lemma seq_block_smaller_all':
-"seq_block (a # xs) \<Longrightarrow>
-(\<forall>x \<in> set xs. fst a < fst x)"
-apply(clarsimp)
-apply(subgoal_tac "\<exists>ys zs. xs = ys @ (aa, b) # zs")
- apply(clarify)
- apply(simp add: seq_block_smaller)
-apply(thin_tac "seq_block _")
-apply(induction xs; simp)
-apply(erule disjE)
- apply(fastforce)
-apply(drule_tac x="aa" and y=b in meta_spec2; clarsimp)
-apply(rule_tac x="(a, b) # ys" in exI; simp)
-done
-
-lemma ind_in_para_aux_bb:
-"(n,js,t) \<in> set (aux_basic_block xs ys) \<Longrightarrow>
-\<exists>x\<in>set(ys@xs). fst x = n"
-apply(induction xs arbitrary: ys)
- apply(case_tac ys; simp add: aux_basic_block.simps)
-apply(simp add: aux_basic_block.simps Let_def)
-apply(clarsimp; rename_tac nx ni xs ys)
-apply(case_tac "reg_inst ni \<and> ni \<noteq> Pc JUMPDEST")
- apply(simp split: reg_inst_splits; fastforce)
-apply(case_tac "ni = Pc JUMPDEST")
- apply(simp split: reg_inst_splits; case_tac ys; simp add: block_pt_def)
-  apply(fastforce)
- apply(drule_tac x="[(nx, Pc JUMPDEST)]" in meta_spec; simp)
-apply(drule meta_spec[where x="[]"])
-apply(case_tac ys; simp add: block_pt_def split: reg_inst_splits)
-apply(erule disjE; simp)+
-done
-
-lemma remdups_id_aux_bb:
-"distinct (map fst (ys@xs)) \<Longrightarrow>
-remdups (aux_basic_block xs ys) = (aux_basic_block xs ys)"
-apply(induction xs arbitrary: ys)
- apply(case_tac ys; simp add: aux_basic_block.simps)
-apply(case_tac ys; simp add: aux_basic_block.simps Let_def)
- apply(erule conjE)+
- apply(case_tac "reg_inst (snd a)")
-  apply(simp split: reg_inst_splits; fastforce)
- apply(cut_tac x="fst a" and xys=xs in map_of_eq_None_iff, drule sym, simp)
- apply(case_tac "snd a"; simp split: reg_inst_splits;
-			rename_tac x; case_tac x; simp add: block_pt_def; rule notI)
-      apply(drule_tac ys="[]" and xs="xs" and n="fst a" and js="[]" in ind_in_para_aux_bb; clarsimp)+
-     apply(drule_tac ys="[]" and xs="xs" and n="fst a" and js="[a]" in ind_in_para_aux_bb; clarsimp)+
-apply(erule conjE)+
-apply(clarsimp)
-apply(rename_tac n i xs ny iy yss)
-apply(case_tac "reg_inst i \<and> i \<noteq> Pc JUMPDEST")
- apply(simp split: reg_inst_splits; fastforce)
-apply(case_tac "i = Pc JUMPDEST")
- apply(clarsimp split: reg_inst_splits if_splits)
- apply(simp add: block_pt_def)
- apply(cut_tac x="ny" and xys=xs in map_of_eq_None_iff, drule sym, simp)
- apply(drule ind_in_para_aux_bb; clarsimp)
-apply(cut_tac x="ny" and xys=xs in map_of_eq_None_iff, drule sym, simp)
-apply(case_tac i; simp split: reg_inst_splits;
-			rename_tac x; case_tac x; simp add: block_pt_def; rule notI)
-     apply(drule_tac ys="[]" and xs="xs" and n="ny" and js="(ny, iy) # yss" in ind_in_para_aux_bb; clarsimp)+
-   apply(cut_tac ys="[]" and xs="xs" and n="ny" and js="(ny, iy) # yss @ [(n, i)]" and t=No in ind_in_para_aux_bb; clarsimp)+
-done
-
-lemma distinct_fst_aux_bb:
-"distinct (map fst (ys@xs)) \<Longrightarrow>
- seq_block (ys@xs) \<Longrightarrow>
- distinct (map v_ind (aux_basic_block xs ys))"
-apply(subst distinct_map)
-apply(rule conjI)
- apply(insert remdups_id_aux_bb[where xs=xs and ys=ys]; simp)
-apply(clarsimp simp add: inj_on_def)
-apply(induction xs arbitrary: ys)
- apply(case_tac ys; simp add: aux_basic_block.simps)
-apply(clarsimp)
-apply(rename_tac m i xs is1 t1 n is2 t2 ys)
-apply(simp add: aux_basic_block.simps Let_def)
-apply(case_tac "reg_inst i \<and> i \<noteq> Pc JUMPDEST")
- apply(drule_tac x=is1 and y=t1 in meta_spec2; drule_tac x=n in meta_spec)
- apply(drule_tac x=is2 and y=t2 in meta_spec2; drule_tac x="ys @ [(m, i)]" in meta_spec)
- apply(simp split: reg_inst_splits)
-apply(case_tac "i = Pc JUMPDEST")
- apply(clarsimp split: reg_inst_splits if_splits)
-  apply(drule_tac x=is1 and y=t1 in meta_spec2; drule_tac x=n in meta_spec)
-  apply(drule_tac x=is2 and y=t2 in meta_spec2; drule_tac x="[(m, Pc JUMPDEST)]" in meta_spec)
-  apply(simp)
- apply(erule disjE; erule disjE)
-		apply(simp)
-	 apply(erule conjE)+
-	 apply(case_tac ys; simp add: block_pt_def)
-	 apply(drule ind_in_para_aux_bb; drule seq_block_smaller_all)
-	 apply(fastforce)
-	apply(erule conjE)+
-	apply(case_tac ys; simp add: block_pt_def)
-	apply(drule ind_in_para_aux_bb; drule seq_block_smaller_all)
-	apply(fastforce)
- apply(drule_tac x=is1 and y=t1 in meta_spec2; drule_tac x=n in meta_spec)
- apply(drule_tac x=is2 and y=t2 in meta_spec2; drule_tac x="[(m, Pc JUMPDEST)]" in meta_spec)
- apply(simp add: seq_block_tl')
-apply(subgoal_tac "\<exists>t zs. (n, is1, t1) \<in> set ((block_pt ys (m, i), ys @zs, t) #
-                 aux_basic_block xs []) \<and>
-								 (n, is2, t2) \<in> set ((block_pt ys (m, i), ys@zs, t) #
-                 aux_basic_block xs [])")
-  defer
-  apply(clarsimp split: reg_inst_splits; fastforce)
-apply(thin_tac "(_,_,_)\<in>set (_)")
-apply(thin_tac "(_,_,_)\<in>set (_)")
-apply(clarsimp)
- apply(erule disjE; erule disjE)
-		apply(clarsimp)
-	 apply(erule conjE)+
-	 apply(case_tac ys; simp add: block_pt_def)
-	  apply(drule ind_in_para_aux_bb; drule seq_block_smaller_all')
-	  apply(fastforce)
-	 apply(drule ind_in_para_aux_bb; drule seq_block_smaller_all'; clarsimp)
-	 apply(subgoal_tac "\<forall>x\<in>set xs. a < fst x")
-		apply(fastforce)
-	 apply(simp)
-	apply(erule conjE)+
-	apply(case_tac ys; simp add: block_pt_def)
-	  apply(drule ind_in_para_aux_bb; drule seq_block_smaller_all')
-	  apply(fastforce)
-	 apply(drule ind_in_para_aux_bb; drule seq_block_smaller_all'; clarsimp)
-	 apply(subgoal_tac "\<forall>x\<in>set xs. a < fst x")
-		apply(fastforce)
-	 apply(simp)
- apply(drule_tac x=is1 and y=t1 in meta_spec2; drule_tac x=n in meta_spec)
- apply(drule_tac x=is2 and y=t2 in meta_spec2; drule_tac x="[]" in meta_spec; simp)
- apply(simp add: seq_block_tl'[where xs="_@[_]"])
-done
-
-lemma re_build_bb:
-"blocks_vertices (build_blocks xs) (blocks_indexes (build_blocks xs)) = build_vertices xs"
-apply(simp add: build_blocks_def Let_def extract_indexes_def)
-apply(rule blocks_vert_rebuild)
-apply(simp add: build_vertices_def add_address_def)
-apply(rule distinct_fst_aux_bb)
- apply(simp add: distinct_add_address)
-apply(simp add: seq_block_add_address)
-done
-
-lemma re_build_address:
-"blocks_pos_insts (blocks_vertices (build_blocks xs) (blocks_indexes (build_blocks xs))) = add_address xs"
-apply(simp add: re_build_bb)
-apply(simp add: build_vertices_def reverse_basic_blocks_add)
-done
-
-lemma jump_i_ends_block:
-"seq_block (ys@xs) \<Longrightarrow>
- (t=Jump \<and> i=JUMP) \<or> (t=Jumpi \<and> i=JUMPI) \<Longrightarrow>
- (n, insts, t) \<in> set (aux_basic_block xs ys) \<Longrightarrow>
- (n + inst_size_list insts, Pc i) \<in> set xs"
- apply(induction xs arbitrary: ys)
-  apply(case_tac ys; simp add: aux_basic_block.simps)
- apply(clarsimp simp add: aux_basic_block.simps Let_def)
- apply(case_tac "reg_inst b \<and> b \<noteq> Pc JUMPDEST")
-  apply(drule_tac x="ys @ [(a, b)]" in meta_spec)
-  apply(simp split: reg_inst_splits)
- apply(case_tac "b=Pc JUMPDEST")
-  apply(case_tac ys)
-	 apply(simp; drule_tac x="[(a, b)]" in meta_spec; simp)
-  apply(simp; drule_tac x="[(a, b)]" in meta_spec; simp add: seq_block_tl'[where xs="_#_"])
-  apply(erule disjE; simp)
- apply(drule_tac x="[]" in meta_spec)
- apply(drule meta_mp)
-  apply(subgoal_tac "seq_block ((a, b) # xs)")
-	 apply(simp add: seq_block_tl)
-  apply(simp add: seq_block_tl')
- apply(simp split: reg_inst_splits; erule disjE; simp)
-  apply(erule disjE; simp)
-  apply(case_tac ys; simp add: block_pt_def seq_block_sumC)
- apply(erule disjE; simp)
- apply(case_tac ys; simp add: block_pt_def seq_block_sumC)
-done
-
-lemma jumps_end_block:
-"(t=Jump \<and> i=JUMP) \<or> (t=Jumpi \<and> i=JUMPI) \<Longrightarrow>
- blocks_list (build_blocks bytecode) n = Some (insts, t) \<Longrightarrow>
- program_content (program_from_blocks (build_blocks bytecode))
-  (n + inst_size_list insts) =
- Some (Pc i)"
- apply(simp add: program_from_blocks_def blocks_content_def)
- apply(simp add: re_build_address)
- apply(simp add: build_blocks_def Let_def)
- apply(simp add: build_vertices_def)
- apply(insert map_of_eq_Some_iff[where xys="add_address bytecode" and x="n + inst_size_list insts"
- and y="Pc i"])
- apply(drule meta_mp)
-  apply(simp add: add_address_def distinct_add_address)
- apply(simp add: add_address_def)
- apply(drule map_of_SomeD)
-	apply(subst jump_i_ends_block[where ys="[]"]; simp)
-  apply(simp add: seq_block_add_address)
-done
-
 (* Main theorem *)
 
 lemma wf_build_blocks:
 "fst (last (add_address bytecode)) < 2^256 \<Longrightarrow>
 wf_blocks (build_blocks bytecode)"
  apply(simp add: wf_blocks_def)
+ apply(rule conjI)
+  prefer 2
+  apply(simp add: build_blocks_def Let_def)
  apply(clarsimp)
  apply(rule conjI)
   apply(clarsimp; rule conjI)
@@ -870,7 +436,6 @@ wf_blocks (build_blocks bytecode)"
      apply(cut_tac x=a and y=b in bound_add_address'[where xs=bytecode and k=0]; simp)
     apply(simp)+
  apply(thin_tac "_ < _")
- apply(simp add: jumps_end_block)
  apply(rule conjI)
   apply(simp add: build_blocks_def Let_def build_vertices_def)
   apply(rule impI)
@@ -882,5 +447,82 @@ wf_blocks (build_blocks bytecode)"
  apply(drule map_of_SomeD)
  apply(drule block_no; simp add: reg_block_def)
 done
+
+(* Check that we can rebuild the initial list of instructions from basic blocks *)
+fun inst_size_list::"pos_inst list \<Rightarrow> int" where
+"inst_size_list [] = 0"
+| "inst_size_list (x#xs) = inst_size (snd x) + inst_size_list xs"
+
+lemma seq_block_sumC:
+"seq_block ((i,j) # list @ (a, b) # xs) \<Longrightarrow>
+ i + (inst_size j + inst_size_list list) = a"
+apply(induction list arbitrary: i j; clarsimp)
+ apply(simp add: seq_block.simps)
+apply(simp add: seq_block.simps)
+apply(fastforce)
+done
+
+fun rebuild_with_add :: "vertices \<Rightarrow> pos_inst list" where
+ "rebuild_with_add [] = []"
+| "rebuild_with_add ((n,b,Jump)#q) = b@[(n+inst_size_list b,Pc JUMP)] @ (rebuild_with_add q)"
+| "rebuild_with_add ((n,b,Jumpi)#q) = b@[(n+inst_size_list b,Pc JUMPI)] @ (rebuild_with_add q)"
+| "rebuild_with_add ((n,b,_)#q) = b @ (rebuild_with_add q)"
+
+lemma rev_rebuild_with_add_aux:
+notes if_split[split del]
+shows
+"seq_block (b@c) \<Longrightarrow>
+rebuild_with_add (aux_basic_block c b) =
+    b@c"
+apply(induction c arbitrary: b)
+  apply(case_tac b; simp add: aux_basic_block.simps)
+apply(simp add: aux_basic_block.simps Let_def)
+apply(case_tac "reg_inst (snd a) \<and> snd a \<noteq> Pc JUMPDEST")
+ apply(simp split: reg_inst_splits)
+ apply(drule conjunct1; rule conjI; rule allI; clarify; rule conjI)
+  apply(clarsimp)+
+ apply(rule conjI; clarsimp)
+apply(case_tac "snd a = Pc JUMPDEST"; clarsimp)
+ apply(simp split: if_splits)
+ apply(drule_tac x="[(a, Pc JUMPDEST)]" in meta_spec)
+ apply(simp add: seq_block_tl')
+apply(drule_tac x="[]" in meta_spec)
+apply(drule meta_mp)
+apply(simp add: seq_block_tl'[where xs="_ @ [(_,_)]"])
+apply(case_tac b; simp)
+ apply(rename_tac x; case_tac x; simp add: block_pt_def; case_tac ba; simp add: seq_block_sumC)+
+done
+  
+lemma rev_rebuild_with_add:
+"rebuild_with_add (all_blocks (build_blocks c)) = add_address c"
+apply(simp add: build_blocks_def Let_def)
+apply(simp add: build_vertices_def)
+apply(subst rev_rebuild_with_add_aux)
+ apply(simp add: seq_block_add_address add_address_def)
+apply(simp)
+done
+
+fun reconstruct_bytecode :: "vertices \<Rightarrow> inst list" where
+ "reconstruct_bytecode [] = []"
+| "reconstruct_bytecode ((n,b,Jump)#q) = (map snd b)@[Pc JUMP] @ (reconstruct_bytecode q)"
+| "reconstruct_bytecode ((n,b,Jumpi)#q) = (map snd b)@[Pc JUMPI] @ (reconstruct_bytecode q)"
+| "reconstruct_bytecode ((n,b,_)#q) = (map snd b) @ (reconstruct_bytecode q)"
+
+lemma rev_basic_blocks: "reconstruct_bytecode (aux_basic_block i b) = (map snd b)@(map snd i)"
+apply(induction i arbitrary: b)
+apply(case_tac b)
+apply(auto simp: Let_def aux_basic_block.simps split: reg_inst_splits)
+done
+
+lemma remove_address:
+"map snd (add_address' i k) = i"
+by(induction i arbitrary: k; simp)
+
+lemma reverse_basic_blocks: "reconstruct_bytecode (build_vertices i) = i"
+apply(simp add: rev_basic_blocks build_vertices_def add_address_def remove_address)
+done
+
+definition blocks_insts :: "basic_blocks \<Rightarrow> pos_inst set" where
+"blocks_insts b = set (rebuild_with_add (all_blocks b))"
 
 end
